Moved remaining stuff to Finite_Tensor_Product.

Axioms_Quantum.thy
@@ -175,136 +175,8 @@ abbreviation tensor_maps :: \<open>'a::finite domain_end \<Rightarrow> 'b::finit
 lemma tensor_2hom: \<open>maps_2hom tensor_maps\<close>
   by (simp add: tensor_op_cbilinear)
 
-(* TODO: move tensor stuff into Finite_Tensor_Product *)
-
-
-definition tensor_lift :: \<open>('a::finite, 'b::finite, 'c) maps_2hom \<Rightarrow> (('a\<times>'b, 'c) maps_hom)\<close> where
-  "tensor_lift F2 = (SOME G. clinear G \<and> (\<forall>a b. G (tensor_maps a b) = F2 a b))"
-
-lemma assumes "maps_2hom F2"
-  shows tensor_lift_hom: "maps_hom (tensor_lift F2)"
-  and tensor_existence:  \<open>(\<lambda>a b. tensor_lift F2 (tensor_maps a b)) = F2\<close>
-proof -
-  define F2' t4 \<phi> where
-    \<open>F2' = tensor_lift F2\<close> and
-    \<open>t4 = (\<lambda>(i,j,k,l). tensor_maps (butterket i j) (butterket k l))\<close> and
-    \<open>\<phi> m = (let (i,j,k,l) = inv t4 m in F2 (butterket i j) (butterket k l))\<close> for m
-  have t4inj: "x = y" if "t4 x = t4 y" for x y
-  proof (rule ccontr)
-    obtain i  j  k  l  where x: "x = (i,j,k,l)" by (meson prod_cases4) 
-    obtain i' j' k' l' where y: "y = (i',j',k',l')" by (meson prod_cases4) 
-    have 1: "bra (i,k) *\<^sub>V t4 x *\<^sub>V ket (j,l) = 1"
-      by (auto simp: bra_def t4_def x tensor_op_state butterfly_def' times_applyOp ket_Kronecker_delta_eq
-               simp flip: tensor_ell2_ket)
-    assume \<open>x \<noteq> y\<close>
-    then have 2: "bra (i,k) *\<^sub>V t4 y *\<^sub>V ket (j,l) = 0"
-      by (auto simp: bra_def t4_def x y tensor_op_state butterfly_def' times_applyOp ket_Kronecker_delta_neq
-               simp flip: tensor_ell2_ket)
-    from 1 2 that
-    show False
-      by auto
-  qed
-  have \<open>\<phi> (tensor_maps (butterket i j) (butterket k l)) = F2 (butterket i j) (butterket k l)\<close> for i j k l
-    apply (subst asm_rl[of \<open>tensor_maps (butterket i j) (butterket k l) = t4 (i,j,k,l)\<close>])
-     apply (simp add: t4_def)
-    by (auto simp add: injI t4inj inv_f_f \<phi>_def)
-
-  have *: \<open>range t4 = {tensor_op (butterket i j) (butterket k l) |i j k l. True}\<close>
-    apply (auto simp: case_prod_beta t4_def)
-    using image_iff by fastforce
-
-  have "cblinfun_extension_exists (range t4) \<phi>"
-    apply (rule cblinfun_extension_exists_finite)
-    apply auto unfolding * 
-    using cindependent_tensor_op
-    using cspan_tensor_op
-    by auto
-
-  then obtain G where G: \<open>G *\<^sub>V (t4 (i,j,k,l)) = F2 (butterket i j) (butterket k l)\<close> for i j k l
-    apply atomize_elim
-    unfolding cblinfun_extension_exists_def
-    apply auto
-    by (metis (no_types, lifting) t4inj \<phi>_def f_inv_into_f rangeI split_conv)
-
-  have *: \<open>G *\<^sub>V tensor_maps (butterket i j) (butterket k l) = F2 (butterket i j) (butterket k l)\<close> for i j k l
-    using G by (auto simp: t4_def)
-  have *: \<open>G *\<^sub>V tensor_maps a (butterket k l) = F2 a (butterket k l)\<close> for a k l
-    apply (rule complex_vector.linear_eq_on_span[where g=\<open>\<lambda>a. F2 a _\<close> and B=\<open>{butterket k l|k l. True}\<close>])
-    unfolding linfun_cspan
-    using * apply (auto intro!: linear_compose[unfolded o_def, where f=\<open>\<lambda>a. tensor_maps a _\<close> and g=\<open>(*\<^sub>V) G\<close>])
-    apply (metis cbilinear_def tensor_op_cbilinear)
-    apply (simp add: cblinfun_apply_add clinearI)
-    using assms unfolding cbilinear_def by blast
-  have G_F2: \<open>G *\<^sub>V tensor_maps a b = F2 a b\<close> for a b
-    apply (rule complex_vector.linear_eq_on_span[where g=\<open>F2 a\<close> and B=\<open>{butterket k l|k l. True}\<close>])
-    unfolding linfun_cspan
-    using * apply (auto simp: cblinfun_apply_add clinearI
-                        intro!: linear_compose[unfolded o_def, where f=\<open>tensor_maps a\<close> and g=\<open>(*\<^sub>V) G\<close>])
-    apply (meson cbilinear_def tensor_op_cbilinear)
-    using assms unfolding cbilinear_def by blast
-
-  have \<open>clinear F2' \<and> (\<forall>a b. F2' (tensor_maps a b) = F2 a b)\<close>
-    unfolding F2'_def tensor_lift_def 
-    apply (rule someI[where x=\<open>(*\<^sub>V) G\<close> and P=\<open>\<lambda>G. clinear G \<and> (\<forall>a b. G (tensor_maps a b) = F2 a b)\<close>])
-    using G_F2 by (simp add: cblinfun_apply_add clinearI)
-
-  then show \<open>maps_hom F2'\<close> and \<open>(\<lambda>a b. tensor_lift F2 (tensor_maps a b)) = F2\<close>
-    unfolding F2'_def by auto
-qed
-
-lemma tensor_uniqueness: \<open>maps_2hom F2 \<Longrightarrow> maps_hom F \<Longrightarrow> (\<lambda>a b. F (tensor_maps a b)) = F2 \<Longrightarrow> F = tensor_lift F2\<close>
-  using tensor_extensionality tensor_lift_hom tensor_existence by metis
-
-lift_definition assoc_state0 :: \<open>(('a::finite\<times>'b::finite)\<times>'c::finite) ell2 \<Rightarrow> ('a\<times>('b\<times>'c)) ell2\<close> is
-  \<open>\<lambda>f (a,(b,c)). f ((a,b),c)\<close>
-  by auto
-
-lift_definition assoc_state0' :: \<open>('a::finite\<times>('b::finite\<times>'c::finite)) ell2 \<Rightarrow> (('a\<times>'b)\<times>'c) ell2\<close> is
-  \<open>\<lambda>f ((a,b),c). f (a,(b,c))\<close>
-  by auto
-
-lift_definition assoc_state :: \<open>(('a::finite\<times>'b::finite)\<times>'c::finite) ell2 \<Rightarrow>\<^sub>C\<^sub>L ('a\<times>('b\<times>'c)) ell2\<close>
-  is assoc_state0
-  apply (rule cbounded_linear_finite_ell2)
-  apply (rule clinearI; transfer)
-  by auto
-
-lift_definition assoc_state' :: \<open>('a::finite\<times>('b::finite\<times>'c::finite)) ell2 \<Rightarrow>\<^sub>C\<^sub>L (('a\<times>'b)\<times>'c) ell2\<close> is
-  assoc_state0'
-  apply (rule cbounded_linear_finite_ell2)
-  apply (rule clinearI; transfer)
-  by auto
-
-lemma assoc_state_tensor: \<open>assoc_state *\<^sub>V tensor_ell2 (tensor_ell2 a b) c = tensor_ell2 a (tensor_ell2 b c)\<close>
-  apply (rule cbounded_linear_equal_ket[THEN fun_cong, where x=a])
-    apply (simp add: cblinfun_apply_add clinearI tensor_ell2_add1 tensor_ell2_scaleC1)
-   apply (simp add: clinear_tensor_ell22)
-  apply (rule cbounded_linear_equal_ket[THEN fun_cong, where x=b])
-    apply (simp add: cblinfun_apply_add clinearI tensor_ell2_add1 tensor_ell2_add2 tensor_ell2_scaleC1 tensor_ell2_scaleC2)
-   apply (simp add: clinearI tensor_ell2_add1 tensor_ell2_add2 tensor_ell2_scaleC1 tensor_ell2_scaleC2)
-  apply (rule cbounded_linear_equal_ket[THEN fun_cong, where x=c])
-    apply (simp add: cblinfun_apply_add clinearI tensor_ell2_add2 tensor_ell2_scaleC2)
-   apply (simp add: clinearI tensor_ell2_add2 tensor_ell2_scaleC2)
-  unfolding assoc_state.rep_eq
-  apply transfer
-  by auto
-
-lemma assoc_state'_tensor: \<open>assoc_state' *\<^sub>V tensor_ell2 a (tensor_ell2 b c) = tensor_ell2 (tensor_ell2 a b) c\<close>
-  apply (rule cbounded_linear_equal_ket[THEN fun_cong, where x=a])
-    apply (simp add: cblinfun_apply_add clinearI tensor_ell2_add1 tensor_ell2_scaleC1)
-   apply (simp add: clinearI tensor_ell2_add1 tensor_ell2_scaleC1)
-  apply (rule cbounded_linear_equal_ket[THEN fun_cong, where x=b])
-    apply (simp add: cblinfun_apply_add clinearI tensor_ell2_add1 tensor_ell2_add2 tensor_ell2_scaleC1 tensor_ell2_scaleC2)
-   apply (simp add: clinearI tensor_ell2_add1 tensor_ell2_add2 tensor_ell2_scaleC1 tensor_ell2_scaleC2)
-  apply (rule cbounded_linear_equal_ket[THEN fun_cong, where x=c])
-    apply (simp add: cblinfun_apply_add clinearI tensor_ell2_add2 tensor_ell2_scaleC2)
-   apply (simp add: clinearI tensor_ell2_add2 tensor_ell2_scaleC2)
-  unfolding assoc_state'.rep_eq
-  apply transfer
-  by auto
-
 definition assoc :: \<open>(('a::finite\<times>'b::finite)\<times>'c::finite, 'a\<times>('b\<times>'c)) maps_hom\<close> where
-  \<open>assoc a = assoc_state o\<^sub>C\<^sub>L a o\<^sub>C\<^sub>L assoc_state'\<close>
+  \<open>assoc a = assoc_ell2 o\<^sub>C\<^sub>L a o\<^sub>C\<^sub>L assoc_ell2'\<close>
 
 lemma assoc_hom: \<open>maps_hom assoc\<close>
   unfolding assoc_def
@@ -313,7 +185,7 @@ lemma assoc_hom: \<open>maps_hom assoc\<close>
 lemma assoc_apply: \<open>assoc (tensor_maps (tensor_maps a b) c) = tensor_maps a (tensor_maps b c)\<close>
   apply (rule equal_ket)
   apply (case_tac x)
-  by (simp add: assoc_def times_applyOp tensor_op_state assoc_state_tensor assoc_state'_tensor flip: tensor_ell2_ket)
+  by (simp add: assoc_def times_applyOp tensor_op_ell2 assoc_ell2_tensor assoc_ell2'_tensor flip: tensor_ell2_ket)
 
 
 definition lvalue :: \<open>('a, 'b) maps_hom \<Rightarrow> bool\<close> where
