Finite_Tensor_Products.thy
@@ -78,7 +78,7 @@ proof -
 qed
 
 
-lemma tensor_op_state: "tensor_op A B *\<^sub>V tensor_ell2 \<psi> \<phi> = tensor_ell2 (A *\<^sub>V \<psi>) (B *\<^sub>V \<phi>)"
+lemma tensor_op_ell2: "tensor_op A B *\<^sub>V tensor_ell2 \<psi> \<phi> = tensor_ell2 (A *\<^sub>V \<psi>) (B *\<^sub>V \<phi>)"
 proof -
   have 1: \<open>clinear (\<lambda>a. tensor_op A B *\<^sub>V tensor_ell2 a (ket b))\<close> for b
     by (auto intro!: clinearI simp: tensor_ell2_add1 tensor_ell2_scaleC1 cblinfun_apply_add)
@@ -104,7 +104,7 @@ lemma comp_tensor_op: "(tensor_op a b) o\<^sub>C\<^sub>L (tensor_op c d) = tenso
   c :: "'a::finite ell2 \<Rightarrow>\<^sub>C\<^sub>L 'e ell2" and d :: "'b::finite ell2 \<Rightarrow>\<^sub>C\<^sub>L 'f ell2"
   apply (rule equal_ket)
   apply (rename_tac ij, case_tac ij, rename_tac i j, hypsubst_thin)
-  by (simp flip: tensor_ell2_ket add: tensor_op_state times_applyOp)
+  by (simp flip: tensor_ell2_ket add: tensor_op_ell2 times_applyOp)
 
 
 lemma tensor_op_cbilinear: \<open>cbilinear (tensor_op :: 'a::finite ell2 \<Rightarrow>\<^sub>C\<^sub>L 'b::finite ell2
@@ -113,16 +113,16 @@ proof -
   have \<open>clinear (\<lambda>b::'c ell2 \<Rightarrow>\<^sub>C\<^sub>L 'd ell2. tensor_op a b)\<close> for a :: \<open>'a ell2 \<Rightarrow>\<^sub>C\<^sub>L 'b ell2\<close>
     apply (rule clinearI)
      apply (rule equal_ket, rename_tac ij, case_tac ij, rename_tac i j, hypsubst_thin)
-     apply (simp flip: tensor_ell2_ket add: tensor_op_state apply_cblinfun_distr_left tensor_ell2_add2)
+     apply (simp flip: tensor_ell2_ket add: tensor_op_ell2 apply_cblinfun_distr_left tensor_ell2_add2)
     apply (rule equal_ket, rename_tac ij, case_tac ij, rename_tac i j, hypsubst_thin)
-    by (simp flip: tensor_ell2_ket add: tensor_op_state apply_cblinfun_distr_left tensor_ell2_scaleC2)
+    by (simp flip: tensor_ell2_ket add: tensor_op_ell2 apply_cblinfun_distr_left tensor_ell2_scaleC2)
 
   moreover have \<open>clinear (\<lambda>a::'a::finite ell2 \<Rightarrow>\<^sub>C\<^sub>L 'b::finite ell2. tensor_op a b)\<close> for b :: \<open>'c ell2 \<Rightarrow>\<^sub>C\<^sub>L 'd ell2\<close>
     apply (rule clinearI)
      apply (rule equal_ket, rename_tac ij, case_tac ij, rename_tac i j, hypsubst_thin)
-     apply (simp flip: tensor_ell2_ket add: tensor_op_state apply_cblinfun_distr_left tensor_ell2_add1)
+     apply (simp flip: tensor_ell2_ket add: tensor_op_ell2 apply_cblinfun_distr_left tensor_ell2_add1)
     apply (rule equal_ket, rename_tac ij, case_tac ij, rename_tac i j, hypsubst_thin)
-    by (simp flip: tensor_ell2_ket add: tensor_op_state apply_cblinfun_distr_left tensor_ell2_scaleC1)
+    by (simp flip: tensor_ell2_ket add: tensor_op_ell2 apply_cblinfun_distr_left tensor_ell2_scaleC1)
 
   ultimately show ?thesis
     unfolding cbilinear_def by auto
@@ -132,7 +132,7 @@ qed
 lemma tensor_butter: \<open>tensor_op (butterket i j) (butterket k l) = butterket (i,k) (j,l)\<close>
   for i :: "_" and j :: "_::finite" and k :: "_" and l :: "_::finite"
   apply (rule equal_ket, case_tac x)
-  apply (auto simp flip: tensor_ell2_ket simp: times_applyOp tensor_op_state butterfly_def')
+  apply (auto simp flip: tensor_ell2_ket simp: times_applyOp tensor_op_ell2 butterfly_def')
   by (auto simp: tensor_ell2_scaleC1 tensor_ell2_scaleC2)
 
 lemma cspan_tensor_op: \<open>cspan {tensor_op (butterket i j) (butterket k l)| i (j::_::finite) k (l::_::finite). True} = UNIV\<close>
@@ -163,16 +163,156 @@ qed
 
 lemma tensor_id[simp]: \<open>tensor_op idOp idOp = idOp\<close>
   apply (rule equal_ket, case_tac x)
-  by (simp flip: tensor_ell2_ket add: tensor_op_state)
+  by (simp flip: tensor_ell2_ket add: tensor_op_ell2)
 
 lemma tensor_op_adjoint: \<open>(tensor_op a b)* = tensor_op (a*) (b*)\<close>
   apply (rule cinner_ket_adjointI[symmetric])
-  apply (auto simp flip: tensor_ell2_ket simp: tensor_op_state)
+  apply (auto simp flip: tensor_ell2_ket simp: tensor_op_ell2)
   by (simp add: adjoint_I)
 
 lemma tensor_butterfly[simp]: "tensor_op (butterfly \<psi> \<psi>') (butterfly \<phi> \<phi>') = butterfly (tensor_ell2 \<psi> \<phi>) (tensor_ell2 \<psi>' \<phi>')"
   apply (rule equal_ket, case_tac x)
-  by (simp flip: tensor_ell2_ket add: tensor_op_state butterfly_def'
+  by (simp flip: tensor_ell2_ket add: tensor_op_ell2 butterfly_def'
       times_applyOp tensor_ell2_scaleC1 tensor_ell2_scaleC2)
+
+
+
+definition tensor_lift :: \<open>(('a1::finite ell2 \<Rightarrow>\<^sub>C\<^sub>L 'a2::finite ell2) \<Rightarrow> ('b1::finite ell2 \<Rightarrow>\<^sub>C\<^sub>L 'b2::finite ell2) \<Rightarrow> 'c)
+                        \<Rightarrow> ((('a1\<times>'b1) ell2 \<Rightarrow>\<^sub>C\<^sub>L ('a2\<times>'b2) ell2) \<Rightarrow> 'c::complex_vector)\<close> where
+  "tensor_lift F2 = (SOME G. clinear G \<and> (\<forall>a b. G (tensor_op a b) = F2 a b))"
+
+
+declare [[show_sorts]]
+
+lemma 
+  fixes F2 :: "'a::finite ell2 \<Rightarrow>\<^sub>C\<^sub>L 'b::finite ell2
+            \<Rightarrow> 'c::finite ell2 \<Rightarrow>\<^sub>C\<^sub>L 'd::finite ell2
+            \<Rightarrow> 'e::complex_normed_vector"
+  assumes "cbilinear F2"
+  shows tensor_lift_hom: "clinear (tensor_lift F2)"
+  and tensor_existence:  \<open>(\<lambda>a b. tensor_lift F2 (tensor_op a b)) = F2\<close>
+proof -
+  define F2' t4 \<phi> where
+    \<open>F2' = tensor_lift F2\<close> and
+    \<open>t4 = (\<lambda>(i,j,k,l). tensor_op (butterket i j) (butterket k l))\<close> and
+    \<open>\<phi> m = (let (i,j,k,l) = inv t4 m in F2 (butterket i j) (butterket k l))\<close> for m
+  have t4inj: "x = y" if "t4 x = t4 y" for x y
+  proof (rule ccontr)
+    obtain i  j  k  l  where x: "x = (i,j,k,l)" by (meson prod_cases4) 
+    obtain i' j' k' l' where y: "y = (i',j',k',l')" by (meson prod_cases4) 
+    have 1: "bra (i,k) *\<^sub>V t4 x *\<^sub>V ket (j,l) = 1"
+      by (auto simp: bra_def t4_def x tensor_op_ell2 butterfly_def' times_applyOp ket_Kronecker_delta_eq
+               simp flip: tensor_ell2_ket)
+    assume \<open>x \<noteq> y\<close>
+    then have 2: "bra (i,k) *\<^sub>V t4 y *\<^sub>V ket (j,l) = 0"
+      by (auto simp: bra_def t4_def x y tensor_op_ell2 butterfly_def' times_applyOp ket_Kronecker_delta_neq
+               simp flip: tensor_ell2_ket)
+    from 1 2 that
+    show False
+      by auto
+  qed
+  have \<open>\<phi> (tensor_op (butterket i j) (butterket k l)) = F2 (butterket i j) (butterket k l)\<close> for i j k l
+    apply (subst asm_rl[of \<open>tensor_op (butterket i j) (butterket k l) = t4 (i,j,k,l)\<close>])
+     apply (simp add: t4_def)
+    by (auto simp add: injI t4inj inv_f_f \<phi>_def)
+
+  have *: \<open>range t4 = {tensor_op (butterket i j) (butterket k l) |i j k l. True}\<close>
+    apply (auto simp: case_prod_beta t4_def)
+    using image_iff by fastforce
+
+  have "cblinfun_extension_exists (range t4) \<phi>"
+    apply (rule cblinfun_extension_exists_finite)
+    apply auto unfolding * 
+    using cindependent_tensor_op
+    using cspan_tensor_op
+    by auto
+
+  then obtain G where G: \<open>G *\<^sub>V (t4 (i,j,k,l)) = F2 (butterket i j) (butterket k l)\<close> for i j k l
+    apply atomize_elim
+    unfolding cblinfun_extension_exists_def
+    apply auto
+    by (metis (no_types, lifting) t4inj \<phi>_def f_inv_into_f rangeI split_conv)
+
+  have *: \<open>G *\<^sub>V tensor_op (butterket i j) (butterket k l) = F2 (butterket i j) (butterket k l)\<close> for i j k l
+    using G by (auto simp: t4_def)
+  have *: \<open>G *\<^sub>V tensor_op a (butterket k l) = F2 a (butterket k l)\<close> for a k l
+    apply (rule complex_vector.linear_eq_on_span[where g=\<open>\<lambda>a. F2 a _\<close> and B=\<open>{butterket k l|k l. True}\<close>])
+    unfolding linfun_cspan
+    using * apply (auto intro!: linear_compose[unfolded o_def, where f=\<open>\<lambda>a. tensor_op a _\<close> and g=\<open>(*\<^sub>V) G\<close>])
+    apply (metis cbilinear_def tensor_op_cbilinear)
+    apply (simp add: cblinfun_apply_add clinearI)
+    using assms unfolding cbilinear_def by blast
+  have G_F2: \<open>G *\<^sub>V tensor_op a b = F2 a b\<close> for a b
+    apply (rule complex_vector.linear_eq_on_span[where g=\<open>F2 a\<close> and B=\<open>{butterket k l|k l. True}\<close>])
+    unfolding linfun_cspan
+    using * apply (auto simp: cblinfun_apply_add clinearI
+                        intro!: linear_compose[unfolded o_def, where f=\<open>tensor_op a\<close> and g=\<open>(*\<^sub>V) G\<close>])
+    apply (meson cbilinear_def tensor_op_cbilinear)
+    using assms unfolding cbilinear_def by blast
+
+  have \<open>clinear F2' \<and> (\<forall>a b. F2' (tensor_op a b) = F2 a b)\<close>
+    unfolding F2'_def tensor_lift_def 
+    apply (rule someI[where x=\<open>(*\<^sub>V) G\<close> and P=\<open>\<lambda>G. clinear G \<and> (\<forall>a b. G (tensor_op a b) = F2 a b)\<close>])
+    using G_F2 by (simp add: cblinfun_apply_add clinearI)
+
+  then show \<open>clinear F2'\<close> and \<open>(\<lambda>a b. tensor_lift F2 (tensor_op a b)) = F2\<close>
+    unfolding F2'_def by auto
+qed
+
+lemma tensor_uniqueness: 
+  fixes F2 :: "'a::finite ell2 \<Rightarrow>\<^sub>C\<^sub>L 'b::finite ell2
+            \<Rightarrow> 'c::finite ell2 \<Rightarrow>\<^sub>C\<^sub>L 'd::finite ell2
+            \<Rightarrow> 'e::complex_normed_vector"
+  shows \<open>cbilinear F2 \<Longrightarrow> clinear F \<Longrightarrow> (\<lambda>a b. F (tensor_op a b)) = F2 \<Longrightarrow> F = tensor_lift F2\<close>
+  using tensor_extensionality tensor_lift_hom tensor_existence by metis
+
+
+lift_definition assoc_ell20 :: \<open>(('a::finite\<times>'b::finite)\<times>'c::finite) ell2 \<Rightarrow> ('a\<times>('b\<times>'c)) ell2\<close> is
+  \<open>\<lambda>f (a,(b,c)). f ((a,b),c)\<close>
+  by auto
+
+lift_definition assoc_ell20' :: \<open>('a::finite\<times>('b::finite\<times>'c::finite)) ell2 \<Rightarrow> (('a\<times>'b)\<times>'c) ell2\<close> is
+  \<open>\<lambda>f ((a,b),c). f (a,(b,c))\<close>
+  by auto
+
+lift_definition assoc_ell2 :: \<open>(('a::finite\<times>'b::finite)\<times>'c::finite) ell2 \<Rightarrow>\<^sub>C\<^sub>L ('a\<times>('b\<times>'c)) ell2\<close>
+  is assoc_ell20
+  apply (rule cbounded_linear_finite_ell2)
+  apply (rule clinearI; transfer)
+  by auto
+
+lift_definition assoc_ell2' :: \<open>('a::finite\<times>('b::finite\<times>'c::finite)) ell2 \<Rightarrow>\<^sub>C\<^sub>L (('a\<times>'b)\<times>'c) ell2\<close> is
+  assoc_ell20'
+  apply (rule cbounded_linear_finite_ell2)
+  apply (rule clinearI; transfer)
+  by auto
+
+lemma assoc_ell2_tensor: \<open>assoc_ell2 *\<^sub>V tensor_ell2 (tensor_ell2 a b) c = tensor_ell2 a (tensor_ell2 b c)\<close>
+  apply (rule cbounded_linear_equal_ket[THEN fun_cong, where x=a])
+    apply (simp add: cblinfun_apply_add clinearI tensor_ell2_add1 tensor_ell2_scaleC1)
+   apply (simp add: clinear_tensor_ell22)
+  apply (rule cbounded_linear_equal_ket[THEN fun_cong, where x=b])
+    apply (simp add: cblinfun_apply_add clinearI tensor_ell2_add1 tensor_ell2_add2 tensor_ell2_scaleC1 tensor_ell2_scaleC2)
+   apply (simp add: clinearI tensor_ell2_add1 tensor_ell2_add2 tensor_ell2_scaleC1 tensor_ell2_scaleC2)
+  apply (rule cbounded_linear_equal_ket[THEN fun_cong, where x=c])
+    apply (simp add: cblinfun_apply_add clinearI tensor_ell2_add2 tensor_ell2_scaleC2)
+   apply (simp add: clinearI tensor_ell2_add2 tensor_ell2_scaleC2)
+  unfolding assoc_ell2.rep_eq
+  apply transfer
+  by auto
+
+lemma assoc_ell2'_tensor: \<open>assoc_ell2' *\<^sub>V tensor_ell2 a (tensor_ell2 b c) = tensor_ell2 (tensor_ell2 a b) c\<close>
+  apply (rule cbounded_linear_equal_ket[THEN fun_cong, where x=a])
+    apply (simp add: cblinfun_apply_add clinearI tensor_ell2_add1 tensor_ell2_scaleC1)
+   apply (simp add: clinearI tensor_ell2_add1 tensor_ell2_scaleC1)
+  apply (rule cbounded_linear_equal_ket[THEN fun_cong, where x=b])
+    apply (simp add: cblinfun_apply_add clinearI tensor_ell2_add1 tensor_ell2_add2 tensor_ell2_scaleC1 tensor_ell2_scaleC2)
+   apply (simp add: clinearI tensor_ell2_add1 tensor_ell2_add2 tensor_ell2_scaleC1 tensor_ell2_scaleC2)
+  apply (rule cbounded_linear_equal_ket[THEN fun_cong, where x=c])
+    apply (simp add: cblinfun_apply_add clinearI tensor_ell2_add2 tensor_ell2_scaleC2)
+   apply (simp add: clinearI tensor_ell2_add2 tensor_ell2_scaleC2)
+  unfolding assoc_ell2'.rep_eq
+  apply transfer
+  by auto
 
 end
